SmallStepWf.v
@@ -285,6 +285,353 @@ Proof.
   }
 Qed.
 
+Ltac thats_it := eapply update_reg_and_incrpc_wf; eauto.
+Ltac des_op c op op' HINV :=
+  destruct (Ir.Config.get_val c op) as [op' | ]; try (inversion HINV; fail).
+Ltac des_inv v HINV :=
+  destruct (v); try (inversion HINV; fail).
+Ltac try_wf :=
+  des_ifs; try (eapply update_reg_and_incrpc_wf; try eassumption;
+                try reflexivity; try congruence; fail).
+
+Lemma OPAQUED_PTRSZ_PTRSZ:
+  Ir.SmallStep.OPAQUED_PTRSZ = Ir.PTRSZ.
+Proof.
+  unfold Ir.SmallStep.OPAQUED_PTRSZ.
+  unfold Ir.SmallStep.locked.
+  des_ifs.
+Qed.
+
+Lemma PTRSZ_MEMSZ:
+  Nat.shiftl 2 (Ir.PTRSZ - 1) = Ir.MEMSZ.
+Proof. reflexivity. Qed.
+
+Lemma PTRSZ_MEMSZ2:
+  Nat.double (Nat.shiftl 1 (Ir.PTRSZ - 1)) = Ir.MEMSZ.
+Proof. reflexivity. Qed.
+
+Lemma twos_compl_add_lt:
+  forall a b,
+    twos_compl_add a b Ir.PTRSZ < Ir.MEMSZ.
+Proof.
+  unfold twos_compl_add. unfold twos_compl.
+  intros. rewrite PTRSZ_MEMSZ. apply Nat.mod_upper_bound.
+  pose Ir.MEMSZ_pos. omega.
+Qed.
+
+Lemma gep_wf:
+  forall p n t m inb p0
+         (HGEP:gep p n t m inb = Ir.ptr p0)
+         (HMWF:Ir.Memory.wf m)
+         (HPWF:Ir.Config.ptr_wf p m),
+    Ir.Config.ptr_wf p0 m.
+Proof.
+  intros.
+  unfold gep in HGEP.
+  inv HPWF.
+  des_ifs.
+  { exploit H. ss. intros HH. inv HH. inv H2.
+    rewrite Heq in H3. inv H3.
+    split.
+    { intros. inv H2.
+      split.
+      rewrite OPAQUED_PTRSZ_PTRSZ.
+      apply twos_compl_add_lt.
+      eauto.
+    }
+    { intros. ss. }
+  }
+  { exploit H. ss. intros HH. inv HH. inv H2.
+    split.
+    { intros. inv H2. split.
+      rewrite OPAQUED_PTRSZ_PTRSZ. apply twos_compl_add_lt.
+      eauto. }
+    { intros. ss. }
+  }
+  { exploit H0. ss. intros HH.
+    split.
+    { intros. ss. }
+    { intros. inv H1. rewrite OPAQUED_PTRSZ_PTRSZ.
+      apply twos_compl_add_lt. }
+  }
+  { exploit H0. ss. intros HH.
+    split.
+    { intros. ss. }
+    { intros. inv H1. rewrite OPAQUED_PTRSZ_PTRSZ.
+      apply twos_compl_add_lt. }
+  }
+  { exploit H0. ss. intros HH.
+    split.
+    { intros. ss. }
+    { intros. inv H1. rewrite OPAQUED_PTRSZ_PTRSZ.
+      apply twos_compl_add_lt. }
+  }
+Qed.
+
+Lemma firstn_In {X:Type}:
+  forall (l:list X) n x l'
+         (HF:List.firstn n l = l')
+         (HIN:List.In x l'),
+    List.In x l.
+Proof.
+  intros.
+  generalize dependent l.
+  generalize dependent l'.
+  induction n.
+  { intros. simpl in HF. inv HF. inv HIN. }
+  { simpl. intros.
+    destruct l. inv HF. inv HIN.
+    destruct l'; try congruence.
+    inv HF. inv HIN. left. ss.
+    right. eapply IHn. eassumption. ss.
+  }
+Qed.
+
+Lemma skipn_In {X:Type}:
+  forall (l:list X) n x l'
+         (HF:List.skipn n l = l')
+         (HIN:List.In x l'),
+    List.In x l.
+Proof.
+  intros.
+  generalize dependent l'.
+  generalize dependent l.
+  induction n.
+  { intros. simpl in HF. congruence. }
+  { simpl. intros.
+    destruct l. congruence.
+    eapply IHn in HF. right. ss. ss.
+  }
+Qed.
+
+Lemma bytes_In_c:
+  forall mb ofs len byt b
+         (HBYTES:Ir.MemBlock.bytes mb ofs len = byt)
+         (HIN:List.In b byt),
+    List.In b (Ir.MemBlock.c mb).
+Proof.
+  intros.
+  unfold Ir.MemBlock.bytes in HBYTES.
+  rewrite <- HBYTES in HIN.
+  eapply firstn_In in HIN; try ss.
+  eapply skipn_In in HIN; try ss.
+  ss.
+Qed.
+
+Lemma getpbits_ptr_in_byte:
+  forall x p n
+    (HPBITS:Ir.Byte.getpbits x = Some (p, n)),
+    Ir.Config.ptr_in_byte p n x.
+Proof.
+  intros.
+  unfold Ir.Byte.getpbits in HPBITS.
+  unfold Ir.Config.ptr_in_byte.
+  des_ifs.
+  eauto.
+Qed.
+
+Lemma load_val_ptr_wf:
+  forall md st p retty p0
+         (HLOAD:Ir.load_val (Ir.Config.m st) p retty = Ir.ptr p0)
+         (HWF:Ir.Config.wf md st)
+         (HPWF:Ir.Config.ptr_wf p (Ir.Config.m st)),
+    Ir.Config.ptr_wf p0 (Ir.Config.m st).
+Proof.
+  intros.
+  unfold Ir.load_val in HLOAD.
+  des_ifs.
+  unfold Ir.Byte.getptr in Heq.
+  unfold Ir.ty_bytesz in Heq.
+  unfold Ir.ty_bitsz in Heq.
+  unfold Ir.PTRSZ in Heq.
+  simpl in Heq.
+  des_ifs.
+  unfold Ir.load_bytes in Heq1.
+  des_ifs.
+  dup Heq.
+  apply Ir.get_deref_singleton in Heq4. inv Heq4; try congruence.
+  inv H. inv H0. inv H. simpl in H1.
+  assert (exists x, l = x::nil).
+  { 
+    destruct l; simpl in Heq0; try( inv Heq0; fail).
+    rewrite Nat.eqb_eq in Heq0.
+    destruct l. simpl in Heq0. eexists. reflexivity.
+    simpl in Heq0. omega.
+  }
+  inv H. simpl in Heq0.
+  simpl in Heq3. des_ifs.
+  inv HWF.
+  exploit wf_ptr_mem.
+  { rewrite H1.  reflexivity. }
+  { eapply bytes_In_c. eassumption.
+    assert (In t0 [t0;x]). left. ss. eapply H. }
+  { eapply getpbits_ptr_in_byte. eassumption. }
+  intros. ss.
+  { inv HWF. ss. }
+  omega.
+Qed.
+
+Lemma store_val_ptr_wf:
+  forall md p0 c p v valty
+         (HWF:Ir.Config.wf md c)
+         (HPWF:Ir.Config.ptr_wf p0 (Ir.Config.m c)),
+  Ir.Config.ptr_wf p0 (Ir.store_val (Ir.Config.m c) p v valty).
+Proof.
+  intros.
+  inv HPWF.
+  destruct p0.
+  { exploit H. ss. intros HH. inv HH. inv H2.
+    split.
+    { intros. inv H2. split. ss.
+      unfold Ir.store_val. des_ifs; eauto.
+      { unfold Ir.store_bytes.
+        des_ifs; eauto.
+        destruct (b =? l) eqn:HEQ.
+        { rewrite Nat.eqb_eq in HEQ. subst b.
+          erewrite Ir.Memory.get_set_id_short; try eassumption.
+          eexists. ss. inv HWF. ss. }
+        { rewrite Ir.Memory.get_set_diff_short. eexists. eassumption.
+          inv HWF. ss. rewrite Nat.eqb_neq in HEQ. congruence. }
+      }
+      { unfold Ir.store_bytes.
+        des_ifs; eauto.
+        destruct (b =? l) eqn:HEQ.
+        { rewrite Nat.eqb_eq in HEQ. subst b.
+          erewrite Ir.Memory.get_set_id_short; try eassumption.
+          eexists. ss. inv HWF. ss. }
+        { rewrite Ir.Memory.get_set_diff_short. eexists. eassumption.
+          inv HWF. ss. rewrite Nat.eqb_neq in HEQ. congruence. }
+      }
+    }
+    { intros. congruence. }
+  }
+  { exploit H0. ss. intros HH.
+    split.
+    { intros. congruence. }
+    { intros. inv H1. ss. }
+  }
+Qed.
+
+(* Lemma: inst_det_step preserves well-formedness of configuration. *)
+Lemma inst_det_step_wf:
+  forall md c c' i e
+         (HWF:Ir.Config.wf md c)
+         (HCUR:Some i = Ir.Config.cur_inst md c)
+         (HNEXT:Some (sr_success e c') = inst_det_step md c),
+    Ir.Config.wf md c'.
+Proof.
+    intros.
+    unfold inst_det_step in HNEXT. (* ibinop. *)
+    rewrite <- HCUR in HNEXT.
+    destruct i as [r retty bopc op1 op2 (* ibinop *)
+                  |r retty ptrty opptr1 opptr2 (* ipsub *)
+                  |r retty opptr opidx inb (* igep *)
+                  |r retty opptr (* iload *)
+                  |valty opval opptr (* istore *)
+                  |(* imalloc *)
+                  |opptr (* ifree *)
+                  |r opval retty (* ibitcast *)
+                  |r opptr retty (* iptrtoint *)
+                  |r opint retty (* iinttoptr *)
+                  |opval (* ievent *)
+                  |r opty op1 op2 (* iicmp_eq *)
+                  |r opty op1 op2 (* iicmp_ule *)
+                  ] eqn:HINST; try (inversion HNEXT; fail).
+    + destruct bopc; try_wf.
+    + (* ipsub. *) unfold psub in HNEXT. try_wf.
+    + (* igep. *) try_wf.
+      eapply update_reg_and_incrpc_wf; try reflexivity.
+      eassumption.
+      intros. eapply gep_wf; try eassumption.
+      inv HWF. assumption. inv HWF. eapply wf_ptr; eassumption.
+    + (* iload. *) try_wf.
+      eapply update_reg_and_incrpc_wf. eassumption. reflexivity.
+      intros. dup HWF. inv HWF.
+      eapply load_val_ptr_wf. eassumption. eassumption.
+      eapply wf_ptr. eassumption.
+    + (* istore. *) try_wf; try (eapply incrpc_wf; try eassumption; try reflexivity; fail).
+      apply incrpc_wf with (c := Ir.Config.update_m c (Ir.store_val (Ir.Config.m c) p v valty)).
+      dup HWF. destruct HWF.
+      split; simpl; try assumption. eapply Ir.store_val_wf. eassumption.
+      eapply Ir.ty_bytesz_pos. congruence.
+      * intros. rewrite Ir.Config.get_val_update_m in HGETVAL.
+        eapply store_val_ptr_wf. eassumption.
+        eapply wf_ptr in HGETVAL. ss.
+      * (* wf_ptr_mem *)
+        admit.
+      * reflexivity.
+    + (* ifree *) try_wf; try (eapply incrpc_wf; try eassumption; try reflexivity; fail).
+      apply incrpc_wf with (c := Ir.Config.update_m c t); try reflexivity.
+      unfold free in Heq0.
+      destruct HWF.
+      des_ifs.
+      * split. eapply Ir.Memory.free_wf. eassumption.
+        rewrite Heq0. unfold Ir.Config.update_m. reflexivity.
+        unfold Ir.Config.cid_to_f in *. des_ifs.
+        intros. apply wf_cid_to_f2. unfold Ir.Config.cid_to_f in *. des_ifs.
+        intros.
+        apply wf_stack with (curcid := curcid) (funid := funid) (curregfile := curregfile).
+        assumption. unfold Ir.Config.cid_to_f in *.
+        unfold Ir.Config.update_m in HIN2. destruct c. simpl in *. assumption.
+        assumption.
+        ++ (* wf_ptr *) admit.
+        ++ (* wf_ptr_mem*) admit.
+      * split. eapply Ir.Memory.free_wf. eassumption.
+        rewrite Heq0. unfold Ir.Config.update_m. reflexivity.
+        unfold Ir.Config.cid_to_f in *. des_ifs.
+        intros. apply wf_cid_to_f2. unfold Ir.Config.cid_to_f in *. des_ifs.
+        intros.
+        apply wf_stack with (curcid := curcid) (funid := funid) (curregfile := curregfile).
+        assumption. unfold Ir.Config.cid_to_f in *.
+        unfold Ir.Config.update_m in HIN2. destruct c. simpl in *. assumption.
+        assumption.
+        ++ admit. (* wf_ptr *)
+        ++ admit. (* wf_ptr_mem *)
+    + (* ibitcast. *) try_wf.
+      eapply update_reg_and_incrpc_wf. eassumption.
+      reflexivity.
+      intros. inv H.
+      inv HWF. eapply wf_ptr. eassumption.
+    + (* iptrtoint. *) try_wf.
+    + (* iinttoptr *) try_wf.
+      eapply update_reg_and_incrpc_wf; try eassumption.
+      reflexivity.
+      intros. inv H.
+      split. intros. congruence.
+      intros. inv H. 
+    + (* ievent *)
+      rename HNEXT into H2. simpl in H2.
+      des_op c opval opv H2. des_inv opv H2.
+      inversion H2. eapply incrpc_wf. eassumption. reflexivity.
+    + (* iicmp_eq, det *)
+      rename HNEXT into HC'. simpl in HC'.
+      des_op c op1 op1v HC'.
+      { destruct op1v.
+        - des_op c op2 op2v HC'.
+          destruct op2v; inversion HC'; thats_it. inv HC'. try_wf.
+        - des_op c op2 op2v HC'.
+          destruct op2v; try (inversion HC'; fail).
+          inv HC'. try_wf.
+          destruct (icmp_eq_ptr p p0 (Ir.Config.m c)) eqn:Heq_ptr; try (inversion HC'; fail);
+             inversion HC'; thats_it.
+          inversion HC'. thats_it.
+          inv HC'. try_wf.
+        - inversion HC'. thats_it. }
+      { des_op c op2 op2v HC'.
+        destruct op2v; try (inversion HC'; fail).
+        inversion HC'. thats_it.
+        inv HC'. try_wf. inv HC'. try_wf. inv HC'. try_wf.
+      }
+    + (* iicmp_ule, det *)
+      rename HNEXT into HC'. simpl in HC'.
+      des_op c op1 op1v HC'.
+      { des_inv op1v HC';
+          des_op c op2 op2v HC'; try (inv HC'; try_wf).
+      }
+      { des_ifs; try_wf. }
+Qed.*)
+Admitted.
+
 
 
 
